%points: 6
Using the theorems of switching algebra, simplify the following logic functions to a sum of of products representation.\\ \\
(a) $F=X' \cdot Y \cdot Z + Y \cdot X + X \cdot Y \cdot Z + Z \cdot X \cdot Y$ \\
(b) $F=Z \cdot (X' + Y') + X \cdot Y \cdot Z$ \\

%start answer
%vspace: 12cm
Solution: \\ \\
(a)\\
\begin{tabular}{rll}
  $F$ & $=X' \cdot Y \cdot Z + Y \cdot X + X \cdot Y \cdot Z + Z \cdot X \cdot Y$ &\\
  $F$ & $=Y \cdot Z + Y \cdot X + Z \cdot X \cdot Y$ & (T10)\\
      & $=Y \cdot Z + Y \cdot X$ & (T9)\\
\end{tabular}\\ \\
(b)\\
Note: $X' + Y' = (X \cdot Y)'$ by (T13)\\
\begin{tabular}{rll}
  $F$ & $=Z \cdot (X' + Y') + X \cdot Y \cdot Z$ &\\
      & $=Z$ & (T10)\\
\end{tabular}\\ \\
%end answer
